Split up spec

ZenWithTerms/isabelle/ZenWithTerms.thy
@@ -1,318 +1,30 @@
 theory ZenWithTerms
-  imports "../../common/isabelle/TLA-Utils"
+  imports Spec
 begin
 
-lemma card_insert_le_general: "card A \<le> card (insert x A)"
-proof (cases "finite A")
-  case True thus ?thesis by (intro card_insert_le)
-qed simp
+lemma laTerm_simps[simp]: "laTerm \<lparr> source = nf, dest = nm, term = tm, payload = Join \<lparr> jp_laTerm = tm', jp_laVersion = vn \<rparr> \<rparr> = tm'"
+  by (simp add: laTerm_def)
 
-typedecl Value
-typedecl Node
+lemma laVersion_simps[simp]: "laVersion \<lparr> source = nf, dest = nm, term = tm, payload = Join \<lparr> jp_laTerm = tm', jp_laVersion = vn \<rparr> \<rparr> = vn"
+  by (simp add: laVersion_def)
 
-definition ValidConfigs :: "Node set set"
-  where "ValidConfigs \<equiv> {vs. finite vs \<and> vs \<noteq> {}}"
+lemma version_simps[simp]:
+  "version \<lparr> source = nm, dest = nf, term = tm, payload = PublishRequest \<lparr> prq_version = vn, prq_value = v, prq_config = c, prq_commConf = cc \<rparr> \<rparr> = vn"
+  "version \<lparr> source = nf, dest = nm, term = tm, payload = PublishResponse \<lparr> prs_version = vn  \<rparr> \<rparr> = vn"
+  "version \<lparr> source = nm, dest = nf, term = tm, payload = Commit \<lparr> c_version = vn \<rparr> \<rparr> = vn"
+  by (simp_all add: version_def)
 
-definition modifyAt :: "('a \<Rightarrow> 'b) \<Rightarrow> 'a \<Rightarrow> ('b \<Rightarrow> 'b) \<Rightarrow> ('a \<Rightarrow> 'b)"
-  where "modifyAt f a0 mb a \<equiv> if a = a0 then mb (f a) else f a"
+lemma value_simps[simp]:
+  "value \<lparr> source = nm, dest = nf, term = tm, payload = PublishRequest \<lparr> prq_version = vn, prq_value = v, prq_config = c, prq_commConf = cc \<rparr> \<rparr> = v"
+  by (simp add: value_def)
 
-lemma modifyAt_eq_simp[simp]: "modifyAt f a mb a = mb (f a)" by (simp add: modifyAt_def)
-lemma modifyAt_ne_simp[simp]: "a \<noteq> a0 \<Longrightarrow> modifyAt f a0 mb a = f a" by (simp add: modifyAt_def)
+lemma config_simps[simp]:
+  "config \<lparr> source = nm, dest = nf, term = tm, payload = PublishRequest \<lparr> prq_version = vn, prq_value = v, prq_config = c, prq_commConf = cc \<rparr> \<rparr> = c"
+  by (simp add: config_def)
 
-definition modified :: "('a \<Rightarrow> 'b) stfun \<Rightarrow> 'a \<Rightarrow> ('b \<Rightarrow> 'b) \<Rightarrow> action"
-  where "modified f a mb st \<equiv> f (snd st) = modifyAt (f (fst st)) a mb"
-
-definition updated :: "('a \<Rightarrow> 'b) stfun \<Rightarrow> 'a \<Rightarrow> 'b \<Rightarrow> action"
-  where "updated f a b = modified f a (\<lambda>_. b)"
-
-definition unspecified :: "('a \<Rightarrow> 'b) stfun \<Rightarrow> 'a \<Rightarrow> action"
-  where "unspecified f a st = (\<forall> a'. a' \<noteq> a \<longrightarrow> f (fst st) a' = f (snd st) a')"
-
-record DescendentsEntry =
-  prevT :: nat
-  prevI :: nat
-  nextT :: nat
-  nextI :: nat
-
-record JoinPayload =
-  jp_laTerm     :: nat
-  jp_laVersion  :: nat
-
-record PublishRequestPayload =
-  prq_version  :: nat
-  prq_value    :: Value
-  prq_config   :: "Node set"
-  prq_commConf :: "Node set"
-
-record PublishResponsePayload =
-  prs_version  :: nat
-
-record CommitPayload =
-  c_version  :: nat
-
-datatype Payload
-  = Join            JoinPayload
-  | PublishRequest  PublishRequestPayload
-  | PublishResponse PublishResponsePayload
-  | Commit          CommitPayload
-
-record Message =
-  source  :: Node
-  dest    :: Node
-  "term"  :: nat (* quoting needed because 'term' is a reserved word *)
-  payload :: Payload
-
-definition laTerm    :: "Message \<Rightarrow> nat" where "laTerm     m \<equiv> case payload m of Join jp \<Rightarrow> jp_laTerm     jp"
-definition laVersion :: "Message \<Rightarrow> nat" where "laVersion  m \<equiv> case payload m of Join jp \<Rightarrow> jp_laVersion  jp"
-definition version   :: "Message \<Rightarrow> nat" where "version  m \<equiv> case payload m of
-    PublishRequest  prq \<Rightarrow> prq_version  prq
-  | PublishResponse prs \<Rightarrow> prs_version  prs
-  | Commit          c   \<Rightarrow> c_version    c"
-definition "value"   :: "Message \<Rightarrow> Value" where "value m \<equiv> case payload m of
-    PublishRequest  prq \<Rightarrow> prq_value prq"
-definition config    :: "Message \<Rightarrow> Node set" where "config m \<equiv> case payload m of
-    PublishRequest  prq \<Rightarrow> prq_config prq"
-definition commConf  :: "Message \<Rightarrow> Node set" where "commConf m \<equiv> case payload m of
-    PublishRequest  prq \<Rightarrow> prq_commConf prq"
-
-datatype TermVersion  = TermVersion  nat (* term *) nat (* version  *)
-
-instantiation TermVersion  :: linorder
-begin
-fun less_TermVersion  :: "TermVersion  \<Rightarrow> TermVersion  \<Rightarrow> bool" where
-  "less_TermVersion  (TermVersion  t1 i1) (TermVersion  t2 i2) = (t1 < t2 \<or> (t1 = t2 \<and> i1 < i2))"
-definition less_eq_TermVersion  :: "TermVersion  \<Rightarrow> TermVersion  \<Rightarrow> bool" where
-  "less_eq_TermVersion  ti1 ti2 = (ti1 = ti2 \<or> ti1 < ti2)"
-instance proof
-  fix x y z :: TermVersion
-  obtain tx ix where x: "x = TermVersion  tx ix" by (cases x, auto)
-  obtain ty iy where y: "y = TermVersion  ty iy" by (cases y, auto)
-  obtain tz iz where z: "z = TermVersion  tz iz" by (cases z, auto)
-
-  from x y z
-  show "(x < y) = (x \<le> y \<and> \<not> y \<le> x)" "x \<le> x" "x \<le> y \<Longrightarrow> y \<le> z \<Longrightarrow> x \<le> z"
-    "x \<le> y \<Longrightarrow> y \<le> x \<Longrightarrow> x = y" "x \<le> y \<or> y \<le> x" by (auto simp add: less_eq_TermVersion_def)
-qed
-end
-
-locale ZenWithTerms =
-  (* real variables *)
-  fixes currentTerm                 :: "(Node \<Rightarrow> nat)      stfun"
-  fixes lastCommittedConfiguration  :: "(Node \<Rightarrow> Node set) stfun"
-  fixes lastAcceptedTerm            :: "(Node \<Rightarrow> nat)      stfun"
-  fixes lastAcceptedVersion         :: "(Node \<Rightarrow> nat)      stfun"
-  fixes lastAcceptedValue           :: "(Node \<Rightarrow> Value)    stfun"
-  fixes lastAcceptedConfiguration   :: "(Node \<Rightarrow> Node set) stfun"
-  fixes joinVotes                   :: "(Node \<Rightarrow> Node set) stfun"
-  fixes startedJoinSinceLastReboot  :: "(Node \<Rightarrow> bool)     stfun"
-  fixes electionWon                 :: "(Node \<Rightarrow> bool)     stfun"
-  fixes lastPublishedConfiguration  :: "(Node \<Rightarrow> Node set) stfun"
-  fixes lastPublishedVersion        :: "(Node \<Rightarrow> nat)      stfun"
-  fixes publishVotes                :: "(Node \<Rightarrow> Node set) stfun"
-    (* message history *)
-  fixes messages                    :: "Message set stfun"
-    (* artificial variables *)
-  fixes descendant                  :: "DescendentsEntry set stfun"
-  fixes initialConfiguration        :: "Node set stfun" (* constant *)
-  fixes initialValue                :: "Value stfun" (* constant *)
-  fixes leaderHistory               :: "(nat \<times> Node) set stfun"
-  fixes basedOn                     :: "(TermVersion  \<times> TermVersion) set stfun"
-    (* TODO idea: track last-committed term + version, to link the current state to the proposals *)
-  fixes vars defines "vars \<equiv> LIFT (currentTerm, lastCommittedConfiguration, lastAcceptedTerm,
-      lastAcceptedVersion, lastAcceptedValue, lastAcceptedConfiguration, joinVotes, startedJoinSinceLastReboot,
-      electionWon, lastPublishedConfiguration, lastPublishedVersion, publishVotes, messages, descendant,
-      initialConfiguration, initialValue, leaderHistory, basedOn)"
-    (* IsQuorum predicate *)
-  fixes IsQuorum :: "Node set \<Rightarrow> Node set \<Rightarrow> bool"
-  defines "IsQuorum votes qconfig \<equiv> card (votes \<inter> qconfig) * 2 > card qconfig"
-    (* ElectionWon predicate *)
-  fixes ElectionWon :: "Node \<Rightarrow> Node set \<Rightarrow> stpred"
-  defines "ElectionWon n votes \<equiv> PRED
-    ( IsQuorum<#votes,id<lastCommittedConfiguration,#n>>
-    \<and> IsQuorum<#votes,id<lastAcceptedConfiguration,#n>>
-    )"
-    (* Initial state *)
-  fixes Initial :: stpred
-  defines "Initial \<equiv> PRED
-      (\<forall>n. id<currentTerm,#n> = #0)
-    \<and> (\<forall>n. id<lastCommittedConfiguration,#n> = initialConfiguration) (* agreement on initial configuration *)
-    \<and> (\<forall>n. id<lastAcceptedTerm,#n> = #0)
-    \<and> (\<forall>n. id<lastAcceptedVersion,#n> = #0)
-    \<and> (\<forall>n. id<lastAcceptedValue,#n> = initialValue)
-    \<and> (\<forall>n. id<lastAcceptedConfiguration,#n> = initialConfiguration)
-    \<and> (\<forall>n. id<joinVotes,#n> = #{})
-    \<and> (\<forall>n. id<startedJoinSinceLastReboot,#n> = #False)
-    \<and> (\<forall>n. id<electionWon,#n> = #False)
-    (*\<and> (\<forall>n. id<lastPublishedConfiguration,#n> = initialConfiguration) NB deviation from TLA+ model - this is irrelevant until electionWon, so can leave it unspecified. *)
-    (*\<and> (\<forall>n. id<lastPublishedVersion,#n> = #0)                         NB deviation from TLA+ model - this is irrelevant until electionWon, so can leave it unspecified. *)
-    \<and> (\<forall>n. id<publishVotes,#n> = #{})
-    \<and> messages = #{}
-    \<and> descendant = #{}
-    \<and> initialConfiguration \<in> #ValidConfigs
-    \<and> leaderHistory = #{}
-    \<and> basedOn = #{}"
-    (* HandleStartJoin *)
-    (* Send join request from node n to node nm for term t *)
-  fixes HandleStartJoin :: "Node \<Rightarrow> Node \<Rightarrow> nat \<Rightarrow> action"
-  defines "HandleStartJoin n nm t \<equiv> ACT
-    (id<$currentTerm,#n> < #t
-      \<and> (\<exists> joinRequest. (\<exists> lastAcceptedTerm_n lastAcceptedVersion_n.
-                              #lastAcceptedTerm_n     = id<$lastAcceptedTerm,#n>
-                            \<and> #lastAcceptedVersion_n = id<$lastAcceptedVersion,#n>
-                            \<and> #(joinRequest = \<lparr> source = n, dest = nm, term = t, payload = Join \<lparr> jp_laTerm = lastAcceptedTerm_n, jp_laVersion  = lastAcceptedVersion_n \<rparr> \<rparr>))
-          \<and> updated     currentTerm                n t
-          \<and> unspecified lastPublishedVersion       n (* NB deviation from TLA+ model - this is irrelevant until electionWon, so can leave it unspecified. *)
-          \<and> unspecified lastPublishedConfiguration n (* NB deviation from TLA+ model - this is irrelevant until electionWon, so can leave it unspecified. *)
-          \<and> updated     startedJoinSinceLastReboot n True
-          \<and> updated     electionWon                n False
-          \<and> updated     joinVotes                  n {}
-          \<and> updated     publishVotes               n {}
-          \<and> messages$ = ($messages \<union> #{ joinRequest })
-          \<and> unchanged (lastCommittedConfiguration, lastAcceptedTerm, lastAcceptedVersion, lastAcceptedValue,
-                       lastAcceptedConfiguration, descendant, initialConfiguration,
-                       initialValue, leaderHistory, basedOn)))"
-    (* HandleJoinRequest *)
-    (* node n handles a join request and checks if it has received enough joins (= votes) for its term to be elected as master *)
-  fixes HandleJoinRequest :: "Node \<Rightarrow> Message \<Rightarrow> action"
-  defines "HandleJoinRequest n m \<equiv> ACT
-    ( #(case payload m of Join _ \<Rightarrow> True | _ \<Rightarrow> False)
-    \<and> #(term m) = id<$currentTerm,#n>
-    \<and> id<$startedJoinSinceLastReboot,#n>
-    \<and> ( #(laTerm m) < id<$lastAcceptedTerm,#n>
-      \<or> ( #(laTerm     m) = id<$lastAcceptedTerm,#n>
-        \<and> #(laVersion  m) \<le> id<$lastAcceptedVersion,#n>)) (* TODO is this needed? *)
-    \<and> modified joinVotes   n (insert (source m))
-    \<and> (\<exists> joinVotes_n electionNowWon. #joinVotes_n = id<joinVotes$,#n>
-                                   \<and> #electionNowWon = $(ElectionWon n joinVotes_n)
-          \<and> updated electionWon n electionNowWon)
-    \<and> (if id<$electionWon,#n> = #False \<and> id<electionWon$,#n>
-        then (\<exists> lav. #lav = id<$lastAcceptedVersion,#n>
-                  \<and> updated lastPublishedVersion n lav)
-           \<and> (\<exists> lac. #lac = id<$lastAcceptedConfiguration,#n>
-                  \<and> updated lastPublishedConfiguration n lac) (* NB deviation from TLA+ model in which lastPublishedConfiguration := lastAcceptedConfiguration occurs during HandleStartJoin *)
-        else unchanged (lastPublishedVersion, lastPublishedConfiguration))
-    \<and> (if id<electionWon$,#n> then leaderHistory$ = (insert (term m, n))<$leaderHistory> else unchanged leaderHistory)
-    \<and> unchanged (lastCommittedConfiguration, currentTerm, publishVotes, messages, descendant,
-                 lastAcceptedVersion, lastAcceptedValue, lastAcceptedConfiguration,
-                 lastAcceptedTerm, startedJoinSinceLastReboot, initialConfiguration, initialValue, basedOn))"
-    (* ClientRequest *)
-    (* client causes a cluster state change v with configuration vs *)
-  fixes ClientRequest :: "Node \<Rightarrow> Value \<Rightarrow> Node set \<Rightarrow> action"
-  defines "ClientRequest n v vs \<equiv> ACT
-    ( id<$electionWon,#n>
-    \<and> id<$lastPublishedVersion,#n> = id<$lastAcceptedVersion,#n> (* means we have the last published value / config (useful for CAS operations, where we need to read the previous value first) *)
-    \<and> (#vs \<noteq> id<$lastAcceptedConfiguration,#n> \<longrightarrow> id<$lastCommittedConfiguration,#n> = id<$lastAcceptedConfiguration,#n>) (* only allow reconfiguration if there is not already a reconfiguration in progress *)
-    \<and> (IsQuorum<id<$joinVotes,#n>,#vs>) (* only allow reconfiguration if we have a quorum of (join) votes for the new config *)
-    \<and> (\<exists> newPublishVersion  publishRequests newEntry matchingElems newTransitiveElems
-          currentTerm_n lastCommittedConfiguration_n lastAcceptedTerm_n lastAcceptedVersion_n.
-            #currentTerm_n          = id<$currentTerm,#n>
-          \<and> #lastCommittedConfiguration_n = id<$lastCommittedConfiguration,#n>
-          \<and> #lastAcceptedTerm_n     = id<$lastAcceptedTerm,#n>
-          \<and> #lastAcceptedVersion_n = id<$lastAcceptedVersion,#n>
-
-          \<and> #newPublishVersion  = id<$lastPublishedVersion,#n> + #1
-          \<and> #publishRequests = #(\<Union> ns \<in> UNIV. {
-                \<lparr> source = n, dest = ns, term = currentTerm_n
-                , payload = PublishRequest \<lparr> prq_version  = newPublishVersion
-                                           , prq_value = v
-                                           , prq_config = vs
-                                           , prq_commConf = lastCommittedConfiguration_n \<rparr>\<rparr>})
-          \<and> #newEntry = #\<lparr> prevT = lastAcceptedTerm_n
-                         , prevI = lastAcceptedVersion_n
-                         , nextT = currentTerm_n
-                         , nextI = newPublishVersion  \<rparr>
-          \<and> #matchingElems = (\<lambda>d. { e \<in> d. nextT e = prevT newEntry \<and> nextI e = prevI newEntry})<$descendant>
-          \<and> #newTransitiveElems = #(\<Union> e \<in> matchingElems. {\<lparr> prevT = prevT e, prevI = prevI e, nextT = nextT newEntry, nextI = nextI newEntry \<rparr>})
-
-          \<and> descendant$ = ($descendant \<union> #{newEntry} \<union> #newTransitiveElems)
-          \<and> updated lastPublishedVersion       n newPublishVersion
-          \<and> updated lastPublishedConfiguration n vs
-          \<and> updated publishVotes               n {}
-          \<and> messages$ = ($messages \<union> #publishRequests)
-          \<and> basedOn$ = (insert ( TermVersion  currentTerm_n newPublishVersion
-                                , TermVersion  lastAcceptedTerm_n lastAcceptedVersion_n ))<$basedOn>
-          \<and> unchanged (startedJoinSinceLastReboot, lastCommittedConfiguration, currentTerm, electionWon,
-                      lastAcceptedVersion, lastAcceptedValue, lastAcceptedTerm,
-                      lastAcceptedConfiguration, joinVotes, initialConfiguration, initialValue,
-                      leaderHistory)))"
-    (* HandlePublishRequest *)
-    (* handle publish request m on node n *)
-  fixes HandlePublishRequest :: "Node \<Rightarrow> Message \<Rightarrow> action"
-  defines "HandlePublishRequest n m \<equiv> ACT
-    ( #(case payload m of PublishRequest _ \<Rightarrow> True | _ \<Rightarrow> False)
-    \<and> #(term m) = id<$currentTerm,#n>
-    \<and> ((#(term m) = id<$lastAcceptedTerm,#n>) \<longrightarrow> (id<$lastAcceptedVersion,#n> < #(version m)))
-    \<and> updated lastAcceptedTerm           n (term     m)
-    \<and> updated lastAcceptedVersion        n (version  m)
-    \<and> updated lastAcceptedValue          n (value    m)
-    \<and> updated lastAcceptedConfiguration  n (config   m)
-    \<and> updated lastCommittedConfiguration n (commConf m)
-    \<and> messages$ = (insert \<lparr> source = n, dest = source m, term = term m
-                          , payload = PublishResponse \<lparr> prs_version  = version m \<rparr> \<rparr>)<$messages>
-    \<and> unchanged (startedJoinSinceLastReboot, currentTerm, descendant, electionWon, lastPublishedVersion, lastPublishedConfiguration, joinVotes,
-                  publishVotes, initialConfiguration, initialValue, leaderHistory, basedOn))"
-    (* HandlePublishResponse *)
-    (* node n commits a change *)
-  fixes HandlePublishResponse :: "Node \<Rightarrow> Message \<Rightarrow> action"
-  defines "HandlePublishResponse n m \<equiv> ACT
-    ( id<$electionWon,#n>
-    \<and> #(case payload m of PublishResponse _ \<Rightarrow> True | _ \<Rightarrow> False)
-    \<and> #(term     m) = id<$currentTerm,#n>
-    \<and> #(version  m) = id<$lastPublishedVersion,#n>
-    \<and> modified publishVotes n (insert (source m))
-    \<and> (if IsQuorum<id<publishVotes$,#n>,id<$lastCommittedConfiguration,#n>>
-        \<and> IsQuorum<id<publishVotes$,#n>,id<$lastPublishedConfiguration,#n>>
-        then (\<exists> commitRequests currentTerm_n lastPublishedVersion_n.
-                  #lastPublishedVersion_n = id<$lastPublishedVersion,#n>
-                \<and> #commitRequests = #(\<Union> ns \<in> UNIV. {
-                        \<lparr> source = n, dest = ns, term = term m
-                        , payload = Commit \<lparr> c_version  = version  m \<rparr> \<rparr>})
-                \<and> messages$ = ($messages \<union> #commitRequests))
-        else unchanged messages)
-    \<and> unchanged (startedJoinSinceLastReboot, lastCommittedConfiguration, currentTerm, electionWon, descendant,
-                   lastAcceptedVersion, lastAcceptedValue, lastAcceptedTerm, lastAcceptedConfiguration,
-                   lastPublishedVersion, lastPublishedConfiguration, joinVotes, initialConfiguration, initialValue, leaderHistory, basedOn))"
-    (* HandleCommitRequest *)
-    (* apply committed configuration to node n *)
-  fixes HandleCommitRequest :: "Node \<Rightarrow> Message \<Rightarrow> action"
-  defines "HandleCommitRequest n m \<equiv> ACT
-    ( #(case payload m of Commit _ \<Rightarrow> True | _ \<Rightarrow> False)
-    \<and> #(term     m) = id<$currentTerm,#n>
-    \<and> #(term     m) = id<$lastAcceptedTerm,#n>
-    \<and> #(version  m) = id<$lastAcceptedVersion,#n>
-    \<and> (\<exists> lastAcceptedConfiguration_n. #lastAcceptedConfiguration_n = id<$lastAcceptedConfiguration,#n>
-          \<and> updated lastCommittedConfiguration n lastAcceptedConfiguration_n)
-    \<and> unchanged (currentTerm, joinVotes, messages, lastAcceptedTerm, lastAcceptedValue, startedJoinSinceLastReboot,
-                 descendant, electionWon, lastAcceptedConfiguration, lastAcceptedVersion,
-                 lastPublishedVersion, lastPublishedConfiguration, publishVotes, initialConfiguration, initialValue, leaderHistory, basedOn))"
-    (* RestartNode *)
-    (* crash/restart node n (loses ephemeral state) *)
-  fixes RestartNode :: "Node \<Rightarrow> action"
-  defines "RestartNode n \<equiv> ACT
-    ( updated     electionWon                n False
-    \<and> updated     startedJoinSinceLastReboot n False
-    \<and> updated     joinVotes                  n {}
-    \<and> unspecified lastPublishedVersion       n (* NB deviation from TLA+ model - this is irrelevant until electionWon, so can leave it unspecified. *)
-    \<and> unspecified lastPublishedConfiguration n (* NB deviation from TLA+ model - this is irrelevant until electionWon, so can leave it unspecified. *)
-    \<and> updated     publishVotes               n {}
-    \<and> unchanged (messages, lastAcceptedVersion, currentTerm, lastCommittedConfiguration, descendant,
-                 lastAcceptedTerm, lastAcceptedValue, lastAcceptedConfiguration, initialConfiguration,
-                 initialValue, leaderHistory, basedOn))"
-    (* Next *)
-    (* next-step relation *)
-  fixes Next :: action
-  defines "Next \<equiv> ACT
-    ( (\<exists> n nm tm. HandleStartJoin n nm tm) (* NB deviation from TLA+ model: here we try arbitrary terms *)
-    \<or> (\<exists> m. #m \<in> $messages \<and> HandleJoinRequest (dest m) m)
-    \<or> (\<exists> n v vs. #vs \<in> #ValidConfigs \<and> ClientRequest n v vs)
-    \<or> (\<exists> m. #m \<in> $messages \<and> HandlePublishRequest  (dest m) m)
-    \<or> (\<exists> m. #m \<in> $messages \<and> HandlePublishResponse (dest m) m)
-    \<or> (\<exists> m. #m \<in> $messages \<and> HandleCommitRequest   (dest m) m)
-    \<or> (\<exists> n. RestartNode n))"
-    (* Spec *)
-    (* Complete specification *)
-  fixes Spec :: temporal
-  defines "Spec \<equiv> TEMP Init Initial \<and> \<box>[Next]_vars"
+lemma commConf_simps[simp]:
+  "commConf \<lparr> source = nm, dest = nf, term = tm, payload = PublishRequest \<lparr> prq_version = vn, prq_value = v, prq_config = c, prq_commConf = cc \<rparr> \<rparr> = cc"
+  by (simp add: commConf_def)
 
 context ZenWithTerms
 begin
@@ -1805,7 +1517,7 @@ proof -
       from prem hyp1 have "\<exists>mp\<in>messages s. isPublishResponse mp \<and> term mc = term mp \<and> version mc = version mp"
       proof (unfold HandlePublishResponse_Quorum, elim UnE UnionE rangeE, simp_all)
         fix n
-        from pr show "\<exists>mp\<in>messages s. isPublishResponse mp \<and> currentTerm s nm = term mp \<and> version \<lparr>source = nm, dest = n, term = currentTerm s nm, payload = Commit \<lparr>c_version = lastPublishedVersion s nm\<rparr>\<rparr> = version mp"
+        from pr show "\<exists>mp\<in>messages s. isPublishResponse mp \<and> currentTerm s nm = term mp \<and> lastPublishedVersion s nm = version mp"
           by (intro bexI [where x = "\<lparr>source = nf, dest = nm, term = currentTerm s nm, payload = PublishResponse \<lparr>prs_version = lastPublishedVersion s nm\<rparr>\<rparr>"], auto simp add: isPublishResponse_def version_def)
       qed
       thus ?thesis by (auto simp add: HandlePublishResponse_Quorum)
