ZenWithTerms/isabelle/Preliminaries.thy
@@ -1,0 +1,98 @@
+theory Preliminaries
+  imports "../../common/isabelle/TLA-Utils"
+begin
+
+lemma card_insert_le_general: "card A \<le> card (insert x A)"
+proof (cases "finite A")
+  case True thus ?thesis by (intro card_insert_le)
+qed simp
+
+typedecl Value
+typedecl Node
+
+definition ValidConfigs :: "Node set set"
+  where "ValidConfigs \<equiv> {vs. finite vs \<and> vs \<noteq> {}}"
+
+definition modifyAt :: "('a \<Rightarrow> 'b) \<Rightarrow> 'a \<Rightarrow> ('b \<Rightarrow> 'b) \<Rightarrow> ('a \<Rightarrow> 'b)"
+  where "modifyAt f a0 mb a \<equiv> if a = a0 then mb (f a) else f a"
+
+lemma modifyAt_eq_simp[simp]: "modifyAt f a mb a = mb (f a)" by (simp add: modifyAt_def)
+lemma modifyAt_ne_simp[simp]: "a \<noteq> a0 \<Longrightarrow> modifyAt f a0 mb a = f a" by (simp add: modifyAt_def)
+
+definition modified :: "('a \<Rightarrow> 'b) stfun \<Rightarrow> 'a \<Rightarrow> ('b \<Rightarrow> 'b) \<Rightarrow> action"
+  where "modified f a mb st \<equiv> f (snd st) = modifyAt (f (fst st)) a mb"
+
+definition updated :: "('a \<Rightarrow> 'b) stfun \<Rightarrow> 'a \<Rightarrow> 'b \<Rightarrow> action"
+  where "updated f a b = modified f a (\<lambda>_. b)"
+
+definition unspecified :: "('a \<Rightarrow> 'b) stfun \<Rightarrow> 'a \<Rightarrow> action"
+  where "unspecified f a st = (\<forall> a'. a' \<noteq> a \<longrightarrow> f (fst st) a' = f (snd st) a')"
+
+record DescendentsEntry =
+  prevT :: nat
+  prevI :: nat
+  nextT :: nat
+  nextI :: nat
+
+record JoinPayload =
+  jp_laTerm     :: nat
+  jp_laVersion  :: nat
+
+record PublishRequestPayload =
+  prq_version  :: nat
+  prq_value    :: Value
+  prq_config   :: "Node set"
+  prq_commConf :: "Node set"
+
+record PublishResponsePayload =
+  prs_version  :: nat
+
+record CommitPayload =
+  c_version  :: nat
+
+datatype Payload
+  = Join            JoinPayload
+  | PublishRequest  PublishRequestPayload
+  | PublishResponse PublishResponsePayload
+  | Commit          CommitPayload
+
+record Message =
+  source  :: Node
+  dest    :: Node
+  "term"  :: nat (* quoting needed because 'term' is a reserved word *)
+  payload :: Payload
+
+definition laTerm    :: "Message \<Rightarrow> nat" where "laTerm     m \<equiv> case payload m of Join jp \<Rightarrow> jp_laTerm     jp"
+definition laVersion :: "Message \<Rightarrow> nat" where "laVersion  m \<equiv> case payload m of Join jp \<Rightarrow> jp_laVersion  jp"
+definition version   :: "Message \<Rightarrow> nat" where "version  m \<equiv> case payload m of
+    PublishRequest  prq \<Rightarrow> prq_version  prq
+  | PublishResponse prs \<Rightarrow> prs_version  prs
+  | Commit          c   \<Rightarrow> c_version    c"
+definition "value"   :: "Message \<Rightarrow> Value" where "value m \<equiv> case payload m of
+    PublishRequest  prq \<Rightarrow> prq_value prq"
+definition config    :: "Message \<Rightarrow> Node set" where "config m \<equiv> case payload m of
+    PublishRequest  prq \<Rightarrow> prq_config prq"
+definition commConf  :: "Message \<Rightarrow> Node set" where "commConf m \<equiv> case payload m of
+    PublishRequest  prq \<Rightarrow> prq_commConf prq"
+
+datatype TermVersion  = TermVersion nat (* term *) nat (* version *)
+
+instantiation TermVersion :: linorder
+begin
+fun less_TermVersion :: "TermVersion \<Rightarrow> TermVersion \<Rightarrow> bool" where
+  "less_TermVersion (TermVersion t1 i1) (TermVersion t2 i2) = (t1 < t2 \<or> (t1 = t2 \<and> i1 < i2))"
+definition less_eq_TermVersion :: "TermVersion \<Rightarrow> TermVersion \<Rightarrow> bool" where
+  "less_eq_TermVersion ti1 ti2 = (ti1 = ti2 \<or> ti1 < ti2)"
+instance proof
+  fix x y z :: TermVersion
+  obtain tx ix where x: "x = TermVersion tx ix" by (cases x, auto)
+  obtain ty iy where y: "y = TermVersion ty iy" by (cases y, auto)
+  obtain tz iz where z: "z = TermVersion tz iz" by (cases z, auto)
+
+  from x y z
+  show "(x < y) = (x \<le> y \<and> \<not> y \<le> x)" "x \<le> x" "x \<le> y \<Longrightarrow> y \<le> z \<Longrightarrow> x \<le> z"
+    "x \<le> y \<Longrightarrow> y \<le> x \<Longrightarrow> x = y" "x \<le> y \<or> y \<le> x" by (auto simp add: less_eq_TermVersion_def)
+qed
+end
+
+end
