ZenWithTerms/isabelle/Spec.thy
@@ -1,0 +1,224 @@
+theory Spec
+  imports Preliminaries
+begin
+
+locale ZenWithTerms =
+  (* real variables *)
+  fixes currentTerm                 :: "(Node \<Rightarrow> nat)      stfun"
+  fixes lastCommittedConfiguration  :: "(Node \<Rightarrow> Node set) stfun"
+  fixes lastAcceptedTerm            :: "(Node \<Rightarrow> nat)      stfun"
+  fixes lastAcceptedVersion         :: "(Node \<Rightarrow> nat)      stfun"
+  fixes lastAcceptedValue           :: "(Node \<Rightarrow> Value)    stfun"
+  fixes lastAcceptedConfiguration   :: "(Node \<Rightarrow> Node set) stfun"
+  fixes joinVotes                   :: "(Node \<Rightarrow> Node set) stfun"
+  fixes startedJoinSinceLastReboot  :: "(Node \<Rightarrow> bool)     stfun"
+  fixes electionWon                 :: "(Node \<Rightarrow> bool)     stfun"
+  fixes lastPublishedConfiguration  :: "(Node \<Rightarrow> Node set) stfun"
+  fixes lastPublishedVersion        :: "(Node \<Rightarrow> nat)      stfun"
+  fixes publishVotes                :: "(Node \<Rightarrow> Node set) stfun"
+    (* message history *)
+  fixes messages                    :: "Message set stfun"
+    (* artificial variables *)
+  fixes descendant                  :: "DescendentsEntry set stfun"
+  fixes initialConfiguration        :: "Node set stfun" (* constant *)
+  fixes initialValue                :: "Value stfun" (* constant *)
+  fixes leaderHistory               :: "(nat \<times> Node) set stfun"
+  fixes basedOn                     :: "(TermVersion \<times> TermVersion) set stfun"
+    (* TODO idea: track last-committed term + version, to link the current state to the proposals *)
+  fixes vars defines "vars \<equiv> LIFT (currentTerm, lastCommittedConfiguration, lastAcceptedTerm,
+      lastAcceptedVersion, lastAcceptedValue, lastAcceptedConfiguration, joinVotes, startedJoinSinceLastReboot,
+      electionWon, lastPublishedConfiguration, lastPublishedVersion, publishVotes, messages, descendant,
+      initialConfiguration, initialValue, leaderHistory, basedOn)"
+    (* IsQuorum predicate *)
+  fixes IsQuorum :: "Node set \<Rightarrow> Node set \<Rightarrow> bool"
+  defines "IsQuorum votes qconfig \<equiv> card (votes \<inter> qconfig) * 2 > card qconfig"
+    (* ElectionWon predicate *)
+  fixes ElectionWon :: "Node \<Rightarrow> Node set \<Rightarrow> stpred"
+  defines "ElectionWon n votes \<equiv> PRED
+    ( IsQuorum<#votes,id<lastCommittedConfiguration,#n>>
+    \<and> IsQuorum<#votes,id<lastAcceptedConfiguration,#n>>
+    )"
+    (* Initial state *)
+  fixes Initial :: stpred
+  defines "Initial \<equiv> PRED
+      (\<forall>n. id<currentTerm,#n> = #0)
+    \<and> (\<forall>n. id<lastCommittedConfiguration,#n> = initialConfiguration) (* agreement on initial configuration *)
+    \<and> (\<forall>n. id<lastAcceptedTerm,#n> = #0)
+    \<and> (\<forall>n. id<lastAcceptedVersion,#n> = #0)
+    \<and> (\<forall>n. id<lastAcceptedValue,#n> = initialValue)
+    \<and> (\<forall>n. id<lastAcceptedConfiguration,#n> = initialConfiguration)
+    \<and> (\<forall>n. id<joinVotes,#n> = #{})
+    \<and> (\<forall>n. id<startedJoinSinceLastReboot,#n> = #False)
+    \<and> (\<forall>n. id<electionWon,#n> = #False)
+    (*\<and> (\<forall>n. id<lastPublishedConfiguration,#n> = initialConfiguration) NB deviation from TLA+ model - this is irrelevant until electionWon, so can leave it unspecified. *)
+    (*\<and> (\<forall>n. id<lastPublishedVersion,#n> = #0)                         NB deviation from TLA+ model - this is irrelevant until electionWon, so can leave it unspecified. *)
+    \<and> (\<forall>n. id<publishVotes,#n> = #{})
+    \<and> messages = #{}
+    \<and> descendant = #{}
+    \<and> initialConfiguration \<in> #ValidConfigs
+    \<and> leaderHistory = #{}
+    \<and> basedOn = #{}"
+    (* HandleStartJoin *)
+    (* Send join request from node n to node nm for term t *)
+  fixes HandleStartJoin :: "Node \<Rightarrow> Node \<Rightarrow> nat \<Rightarrow> action"
+  defines "HandleStartJoin n nm t \<equiv> ACT
+    (id<$currentTerm,#n> < #t
+      \<and> (\<exists> joinRequest. (\<exists> lastAcceptedTerm_n lastAcceptedVersion_n.
+                              #lastAcceptedTerm_n     = id<$lastAcceptedTerm,#n>
+                            \<and> #lastAcceptedVersion_n = id<$lastAcceptedVersion,#n>
+                            \<and> #(joinRequest = \<lparr> source = n, dest = nm, term = t, payload = Join \<lparr> jp_laTerm = lastAcceptedTerm_n, jp_laVersion  = lastAcceptedVersion_n \<rparr> \<rparr>))
+          \<and> updated     currentTerm                n t
+          \<and> unspecified lastPublishedVersion       n (* NB deviation from TLA+ model - this is irrelevant until electionWon, so can leave it unspecified. *)
+          \<and> unspecified lastPublishedConfiguration n (* NB deviation from TLA+ model - this is irrelevant until electionWon, so can leave it unspecified. *)
+          \<and> updated     startedJoinSinceLastReboot n True
+          \<and> updated     electionWon                n False
+          \<and> updated     joinVotes                  n {}
+          \<and> updated     publishVotes               n {}
+          \<and> messages$ = ($messages \<union> #{ joinRequest })
+          \<and> unchanged (lastCommittedConfiguration, lastAcceptedTerm, lastAcceptedVersion, lastAcceptedValue,
+                       lastAcceptedConfiguration, descendant, initialConfiguration,
+                       initialValue, leaderHistory, basedOn)))"
+    (* HandleJoinRequest *)
+    (* node n handles a join request and checks if it has received enough joins (= votes) for its term to be elected as master *)
+  fixes HandleJoinRequest :: "Node \<Rightarrow> Message \<Rightarrow> action"
+  defines "HandleJoinRequest n m \<equiv> ACT
+    ( #(case payload m of Join _ \<Rightarrow> True | _ \<Rightarrow> False)
+    \<and> #(term m) = id<$currentTerm,#n>
+    \<and> id<$startedJoinSinceLastReboot,#n>
+    \<and> ( #(laTerm m) < id<$lastAcceptedTerm,#n>
+      \<or> ( #(laTerm     m) = id<$lastAcceptedTerm,#n>
+        \<and> #(laVersion  m) \<le> id<$lastAcceptedVersion,#n>)) (* TODO is this needed? *)
+    \<and> modified joinVotes   n (insert (source m))
+    \<and> (\<exists> joinVotes_n electionNowWon. #joinVotes_n = id<joinVotes$,#n>
+                                   \<and> #electionNowWon = $(ElectionWon n joinVotes_n)
+          \<and> updated electionWon n electionNowWon)
+    \<and> (if id<$electionWon,#n> = #False \<and> id<electionWon$,#n>
+        then (\<exists> lav. #lav = id<$lastAcceptedVersion,#n>
+                  \<and> updated lastPublishedVersion n lav)
+           \<and> (\<exists> lac. #lac = id<$lastAcceptedConfiguration,#n>
+                  \<and> updated lastPublishedConfiguration n lac) (* NB deviation from TLA+ model in which lastPublishedConfiguration := lastAcceptedConfiguration occurs during HandleStartJoin *)
+        else unchanged (lastPublishedVersion, lastPublishedConfiguration))
+    \<and> (if id<electionWon$,#n> then leaderHistory$ = (insert (term m, n))<$leaderHistory> else unchanged leaderHistory)
+    \<and> unchanged (lastCommittedConfiguration, currentTerm, publishVotes, messages, descendant,
+                 lastAcceptedVersion, lastAcceptedValue, lastAcceptedConfiguration,
+                 lastAcceptedTerm, startedJoinSinceLastReboot, initialConfiguration, initialValue, basedOn))"
+    (* ClientRequest *)
+    (* client causes a cluster state change v with configuration vs *)
+  fixes ClientRequest :: "Node \<Rightarrow> Value \<Rightarrow> Node set \<Rightarrow> action"
+  defines "ClientRequest n v vs \<equiv> ACT
+    ( id<$electionWon,#n>
+    \<and> id<$lastPublishedVersion,#n> = id<$lastAcceptedVersion,#n> (* means we have the last published value / config (useful for CAS operations, where we need to read the previous value first) *)
+    \<and> (#vs \<noteq> id<$lastAcceptedConfiguration,#n> \<longrightarrow> id<$lastCommittedConfiguration,#n> = id<$lastAcceptedConfiguration,#n>) (* only allow reconfiguration if there is not already a reconfiguration in progress *)
+    \<and> (IsQuorum<id<$joinVotes,#n>,#vs>) (* only allow reconfiguration if we have a quorum of (join) votes for the new config *)
+    \<and> (\<exists> newPublishVersion  publishRequests newEntry matchingElems newTransitiveElems
+          currentTerm_n lastCommittedConfiguration_n lastAcceptedTerm_n lastAcceptedVersion_n.
+            #currentTerm_n          = id<$currentTerm,#n>
+          \<and> #lastCommittedConfiguration_n = id<$lastCommittedConfiguration,#n>
+          \<and> #lastAcceptedTerm_n     = id<$lastAcceptedTerm,#n>
+          \<and> #lastAcceptedVersion_n = id<$lastAcceptedVersion,#n>
+
+          \<and> #newPublishVersion  = id<$lastPublishedVersion,#n> + #1
+          \<and> #publishRequests = #(\<Union> ns \<in> UNIV. {
+                \<lparr> source = n, dest = ns, term = currentTerm_n
+                , payload = PublishRequest \<lparr> prq_version  = newPublishVersion
+                                           , prq_value = v
+                                           , prq_config = vs
+                                           , prq_commConf = lastCommittedConfiguration_n \<rparr>\<rparr>})
+          \<and> #newEntry = #\<lparr> prevT = lastAcceptedTerm_n
+                         , prevI = lastAcceptedVersion_n
+                         , nextT = currentTerm_n
+                         , nextI = newPublishVersion  \<rparr>
+          \<and> #matchingElems = (\<lambda>d. { e \<in> d. nextT e = prevT newEntry \<and> nextI e = prevI newEntry})<$descendant>
+          \<and> #newTransitiveElems = #(\<Union> e \<in> matchingElems. {\<lparr> prevT = prevT e, prevI = prevI e, nextT = nextT newEntry, nextI = nextI newEntry \<rparr>})
+
+          \<and> descendant$ = ($descendant \<union> #{newEntry} \<union> #newTransitiveElems)
+          \<and> updated lastPublishedVersion       n newPublishVersion
+          \<and> updated lastPublishedConfiguration n vs
+          \<and> updated publishVotes               n {}
+          \<and> messages$ = ($messages \<union> #publishRequests)
+          \<and> basedOn$ = (insert ( TermVersion  currentTerm_n newPublishVersion
+                                , TermVersion  lastAcceptedTerm_n lastAcceptedVersion_n ))<$basedOn>
+          \<and> unchanged (startedJoinSinceLastReboot, lastCommittedConfiguration, currentTerm, electionWon,
+                      lastAcceptedVersion, lastAcceptedValue, lastAcceptedTerm,
+                      lastAcceptedConfiguration, joinVotes, initialConfiguration, initialValue,
+                      leaderHistory)))"
+    (* HandlePublishRequest *)
+    (* handle publish request m on node n *)
+  fixes HandlePublishRequest :: "Node \<Rightarrow> Message \<Rightarrow> action"
+  defines "HandlePublishRequest n m \<equiv> ACT
+    ( #(case payload m of PublishRequest _ \<Rightarrow> True | _ \<Rightarrow> False)
+    \<and> #(term m) = id<$currentTerm,#n>
+    \<and> ((#(term m) = id<$lastAcceptedTerm,#n>) \<longrightarrow> (id<$lastAcceptedVersion,#n> < #(version m)))
+    \<and> updated lastAcceptedTerm           n (term     m)
+    \<and> updated lastAcceptedVersion        n (version  m)
+    \<and> updated lastAcceptedValue          n (value    m)
+    \<and> updated lastAcceptedConfiguration  n (config   m)
+    \<and> updated lastCommittedConfiguration n (commConf m)
+    \<and> messages$ = (insert \<lparr> source = n, dest = source m, term = term m
+                          , payload = PublishResponse \<lparr> prs_version  = version m \<rparr> \<rparr>)<$messages>
+    \<and> unchanged (startedJoinSinceLastReboot, currentTerm, descendant, electionWon, lastPublishedVersion, lastPublishedConfiguration, joinVotes,
+                  publishVotes, initialConfiguration, initialValue, leaderHistory, basedOn))"
+    (* HandlePublishResponse *)
+    (* node n commits a change *)
+  fixes HandlePublishResponse :: "Node \<Rightarrow> Message \<Rightarrow> action"
+  defines "HandlePublishResponse n m \<equiv> ACT
+    ( id<$electionWon,#n>
+    \<and> #(case payload m of PublishResponse _ \<Rightarrow> True | _ \<Rightarrow> False)
+    \<and> #(term     m) = id<$currentTerm,#n>
+    \<and> #(version  m) = id<$lastPublishedVersion,#n>
+    \<and> modified publishVotes n (insert (source m))
+    \<and> (if IsQuorum<id<publishVotes$,#n>,id<$lastCommittedConfiguration,#n>>
+        \<and> IsQuorum<id<publishVotes$,#n>,id<$lastPublishedConfiguration,#n>>
+        then (\<exists> commitRequests currentTerm_n lastPublishedVersion_n.
+                  #lastPublishedVersion_n = id<$lastPublishedVersion,#n>
+                \<and> #commitRequests = #(\<Union> ns \<in> UNIV. {
+                        \<lparr> source = n, dest = ns, term = term m
+                        , payload = Commit \<lparr> c_version  = version  m \<rparr> \<rparr>})
+                \<and> messages$ = ($messages \<union> #commitRequests))
+        else unchanged messages)
+    \<and> unchanged (startedJoinSinceLastReboot, lastCommittedConfiguration, currentTerm, electionWon, descendant,
+                   lastAcceptedVersion, lastAcceptedValue, lastAcceptedTerm, lastAcceptedConfiguration,
+                   lastPublishedVersion, lastPublishedConfiguration, joinVotes, initialConfiguration, initialValue, leaderHistory, basedOn))"
+    (* HandleCommitRequest *)
+    (* apply committed configuration to node n *)
+  fixes HandleCommitRequest :: "Node \<Rightarrow> Message \<Rightarrow> action"
+  defines "HandleCommitRequest n m \<equiv> ACT
+    ( #(case payload m of Commit _ \<Rightarrow> True | _ \<Rightarrow> False)
+    \<and> #(term     m) = id<$currentTerm,#n>
+    \<and> #(term     m) = id<$lastAcceptedTerm,#n>
+    \<and> #(version  m) = id<$lastAcceptedVersion,#n>
+    \<and> (\<exists> lastAcceptedConfiguration_n. #lastAcceptedConfiguration_n = id<$lastAcceptedConfiguration,#n>
+          \<and> updated lastCommittedConfiguration n lastAcceptedConfiguration_n)
+    \<and> unchanged (currentTerm, joinVotes, messages, lastAcceptedTerm, lastAcceptedValue, startedJoinSinceLastReboot,
+                 descendant, electionWon, lastAcceptedConfiguration, lastAcceptedVersion,
+                 lastPublishedVersion, lastPublishedConfiguration, publishVotes, initialConfiguration, initialValue, leaderHistory, basedOn))"
+    (* RestartNode *)
+    (* crash/restart node n (loses ephemeral state) *)
+  fixes RestartNode :: "Node \<Rightarrow> action"
+  defines "RestartNode n \<equiv> ACT
+    ( updated     electionWon                n False
+    \<and> updated     startedJoinSinceLastReboot n False
+    \<and> updated     joinVotes                  n {}
+    \<and> unspecified lastPublishedVersion       n (* NB deviation from TLA+ model - this is irrelevant until electionWon, so can leave it unspecified. *)
+    \<and> unspecified lastPublishedConfiguration n (* NB deviation from TLA+ model - this is irrelevant until electionWon, so can leave it unspecified. *)
+    \<and> updated     publishVotes               n {}
+    \<and> unchanged (messages, lastAcceptedVersion, currentTerm, lastCommittedConfiguration, descendant,
+                 lastAcceptedTerm, lastAcceptedValue, lastAcceptedConfiguration, initialConfiguration,
+                 initialValue, leaderHistory, basedOn))"
+    (* Next *)
+    (* next-step relation *)
+  fixes Next :: action
+  defines "Next \<equiv> ACT
+    ( (\<exists> n nm tm. HandleStartJoin n nm tm) (* NB deviation from TLA+ model: here we try arbitrary terms *)
+    \<or> (\<exists> m. #m \<in> $messages \<and> HandleJoinRequest (dest m) m)
+    \<or> (\<exists> n v vs. #vs \<in> #ValidConfigs \<and> ClientRequest n v vs)
+    \<or> (\<exists> m. #m \<in> $messages \<and> HandlePublishRequest  (dest m) m)
+    \<or> (\<exists> m. #m \<in> $messages \<and> HandlePublishResponse (dest m) m)
+    \<or> (\<exists> m. #m \<in> $messages \<and> HandleCommitRequest   (dest m) m)
+    \<or> (\<exists> n. RestartNode n))"
+    (* Spec *)
+    (* Complete specification *)
+  fixes Spec :: temporal
+  defines "Spec \<equiv> TEMP Init Initial \<and> \<box>[Next]_vars"
+
+end
